moving common code to auto utils

pulse/lib/steel/pulse/Pulse.Checker.Auto.ElimPure.fst
@@ -56,74 +56,6 @@ let elim_pure_typing (g:env) (p:host_term)
    = admit();
      T_STApp g elim_pure_head (tm_fstar (`(prop))) None (elim_pure_comp p) _ (elim_pure_head_typing g) p_prop
 
-#push-options "--query_stats --fuel 2 --ifuel 2 --split_queries no --z3rlimit_factor 4"
-let continuation_elaborator_with_bind (#g:env) (ctxt:term)
-  (#c1:comp{stateful_comp c1})
-  (#e1:st_term)
-  (e1_typing:st_typing g e1 c1)
-  (ctxt_pre1_typing:tot_typing g (Tm_Star ctxt (comp_pre c1)) Tm_VProp)
-  : T.Tac (x:var { None? (lookup g x) } &
-           continuation_elaborator
-             g (Tm_Star ctxt (comp_pre c1))
-             (extend x (Inl (comp_res c1)) g) (Tm_Star (open_term (comp_post c1) x) ctxt)) =
-
-  let pre1 = comp_pre c1 in
-  let res1 = comp_res c1 in
-  let post1 = comp_post c1 in
-  let ctxt_typing, pre1_typing = star_typing_inversion ctxt_pre1_typing in
-  // let p_prop = Metatheory.pure_typing_inversion pure_typing in
-  let v_eq = VE_Comm g ctxt pre1 in
-  let framing_token : F.frame_for_req_in_ctxt g (Tm_Star ctxt pre1) pre1 = 
-    (| ctxt, ctxt_typing, VE_Comm g pre1 ctxt  |)
-  in
-  let (| c1, e1_typing |) =
-    Pulse.Checker.Framing.apply_frame ctxt_pre1_typing e1_typing framing_token in
-  let (| u_of_1, pre_typing, _, _ |) =
-    Metatheory.(st_comp_typing_inversion (comp_typing_inversion (st_typing_correctness e1_typing))) in
-  let x = fresh g in
-  let b = Inl res1 in
-  let g' = extend x b g in
-  
-  let post1_opened = open_term_nv post1 (v_as_nv x) in
-  let k : continuation_elaborator g (Tm_Star ctxt pre1) g' (Tm_Star post1_opened ctxt) =
-    fun post_hint res ->
-    let (| e2, c2, e2_typing |) = res in
-    if not (stateful_comp c2) // || None? post_hint
-    then T.fail "Unexpected non-stateful comp in continuation elaborate"
-    else (
-      let e2_typing : st_typing g' e2 c2 = e2_typing in
-      let e2_closed = close_st_term e2 x in
-      assume (open_st_term e2_closed x == e2);
-      assert (comp_pre c1 == (Tm_Star ctxt pre1));
-      assert (comp_post c1 == Tm_Star post1 ctxt);
-      assert (comp_pre c2 == Tm_Star post1_opened ctxt);
-      assert (open_term (comp_post c1) x == Tm_Star post1_opened (open_term ctxt x));
-      // ctxt is well-typed, hence ln
-      assume (open_term ctxt x == ctxt);
-      assert (open_term (comp_post c1) x == comp_pre c2);
-      // e2 is well-typed in g, so its fvs should be a subset of g
-      assume (~ (x `Set.mem` freevars_st e2));
-      if x `Set.mem` freevars (comp_post c2)
-      then T.fail "Impossible"
-      else (
-        let t_typing, post_typing =
-          Pulse.Checker.Bind.bind_res_and_post_typing g (st_comp_of_comp c2) x post_hint in
-        let (| e, c, e_typing |) =
-          Pulse.Checker.Bind.mk_bind
-            g (Tm_Star ctxt pre1) 
-            e1 e2_closed c1 c2 (v_as_nv x) e1_typing
-            u_of_1 
-            e2_typing
-            t_typing
-            post_typing
-        in
-        (| e, c, e_typing |)
-      )
-    )
-
-  in
-  (| x, k |)
-
 let elim_one_pure (#g:env) (ctxt:term) (p:term)
                   (ctxt_p_typing:tot_typing g (Tm_Star ctxt (Tm_Pure p)) Tm_VProp)
   : T.Tac (g':env { env_extends g' g } &
@@ -171,67 +103,12 @@ let rec elim_pure_right (#g:env) (#ctxt:term) (ctxt_typing:tot_typing g ctxt Tm_
         extends_env_refl g;
        (| g, ctxt, ctxt_typing, k_elab_unit _ _ |)
 
-module F = Pulse.Checker.Framing
-open Pulse.Checker.VPropEquiv
-
-let rec canon_right_aux (g:env) (vps:list vprop) (f:vprop -> bool)
-  : vps' : list vprop &
-    fvps : list vprop { forall (v:vprop). List.Tot.memP v fvps ==> f v } &
-    vprop_equiv g (list_as_vprop vps) (list_as_vprop (vps' @ fvps)) =
-
-  match vps with
-  | [] -> (| [], [], VE_Refl _ _ |)
-  | hd::rest ->
-    if f hd
-    then begin
-      let (| vps', fvps, v_eq |) = canon_right_aux g rest f in
-      let v_eq
-        : vprop_equiv g (list_as_vprop vps)
-                        (list_as_vprop (hd :: (vps' @ fvps)))
-        = list_as_vprop_ctx g [hd] _ rest (vps' @ fvps) (VE_Refl _ _) v_eq    
-      in  
-      let v_eq
-        : vprop_equiv g (list_as_vprop vps)
-                        (list_as_vprop ((vps'@[hd]) @ fvps))
-        = VE_Trans _ _ _ _ v_eq (VE_Sym _ _ _ (vprop_equiv_swap_equiv _ _ _ hd _ (VE_Refl _ _)))
-      in
-      let v_eq 
-        :  vprop_equiv g (list_as_vprop vps)
-                         (list_as_vprop (vps'@(hd::fvps)))
-        = VE_Trans _ _ _ _ v_eq (VE_Sym _ _ _ (list_as_vprop_assoc _ _ _ _)) in
-      (| vps', hd :: fvps, v_eq |)
-    end
-    else begin
-      let (| vps', pures, v_eq |) = canon_right_aux g rest f in
-      let v_eq = list_as_vprop_ctx g [hd] _ _ _ (VE_Refl _ _) v_eq in
-      (| hd::vps', pures, v_eq |)
-    end
-
-let canon_right (#g:env) (#ctxt:term) (ctxt_typing:tot_typing g ctxt Tm_VProp)
-  (f:vprop -> bool)
-  : (ctxt':term &
-     tot_typing g ctxt' Tm_VProp &
-     continuation_elaborator g ctxt g ctxt')
-  = let ctxt' = canon_vprop ctxt in
-    let (| vps', pures, veq |) = canon_right_aux g (vprop_as_list ctxt) f in
-    let veq : vprop_equiv g ctxt (list_as_vprop (vps'@pures)) =
-        VE_Trans _ _ _ _ (vprop_list_equiv g ctxt) veq
-    in
-    (| _, VP.vprop_equiv_typing_fwd ctxt_typing veq, k_elab_equiv (k_elab_unit _ _) (VE_Refl _ _) veq |)
-
-
-let canon_pure_right (#g:env) (#ctxt:term) (ctxt_typing:tot_typing g ctxt Tm_VProp)
-  : (ctxt':term &
-     tot_typing g ctxt' Tm_VProp &
-     continuation_elaborator g ctxt g ctxt')
-  = canon_right ctxt_typing Tm_Pure?
-
 let elim_pure (#g:env) (#ctxt:term) (ctxt_typing:tot_typing g ctxt Tm_VProp)
    : T.Tac (g':env { env_extends g' g } &
             ctxt':term &
             tot_typing g' ctxt' Tm_VProp &
             continuation_elaborator g ctxt g' ctxt')
-   = let (| ctxt', ctxt'_typing, k |) = canon_pure_right ctxt_typing in
+   = let (| ctxt', ctxt'_typing, k |) = canon_right ctxt_typing Tm_Pure? in
      let (| g', ctxt'', ctxt''_typing, k' |) = elim_pure_right ctxt'_typing in
      extends_env_refl g;
      (| g', ctxt'', ctxt''_typing, k_elab_trans k k' |)
