pulse/lib/steel/pulse/Pulse.Checker.Auto.Util.fsti
@@ -1,4 +1,7 @@
 module Pulse.Checker.Auto.Util
+
+module T = FStar.Tactics
+
 open Pulse.Syntax
 open Pulse.Typing
 open Pulse.Checker.Common
@@ -16,3 +19,19 @@ val k_elab_equiv (#g1 #g2:env) (#ctxt1 #ctxt1' #ctxt2 #ctxt2':term)
                  (d1:vprop_equiv g1 ctxt1 ctxt1')
                  (d2:vprop_equiv g2 ctxt2 ctxt2')
   : continuation_elaborator g1 ctxt1' g2 ctxt2'
+
+val canon_right (#g:env) (#ctxt:term) (ctxt_typing:tot_typing g ctxt Tm_VProp)
+  (f:vprop -> bool)
+  : (ctxt':term &
+     tot_typing g ctxt' Tm_VProp &
+     continuation_elaborator g ctxt g ctxt')
+
+val continuation_elaborator_with_bind (#g:env) (ctxt:term)
+  (#c1:comp{stateful_comp c1})
+  (#e1:st_term)
+  (e1_typing:st_typing g e1 c1)
+  (ctxt_pre1_typing:tot_typing g (Tm_Star ctxt (comp_pre c1)) Tm_VProp)
+  : T.Tac (x:var { None? (lookup g x) } &
+           continuation_elaborator
+             g (Tm_Star ctxt (comp_pre c1))
+             (extend x (Inl (comp_res c1)) g) (Tm_Star (open_term (comp_post c1) x) ctxt))
